update

volume-3-verified-functional-algorithms/ADT.v
@@ -174,7 +174,22 @@ End FunTableExamples.
     Write unit tests to check the operation of [get] and [set]. *)
 
 Module NatFunTableExamples.
-  (* FILL IN HERE *)
+  Module NatVal.
+    Definition V := nat.
+    Definition default := 0.
+  End NatVal.
+
+  Module NatFunTable := FunTable NatVal.
+  Import NatFunTable.
+
+  Example ex1 : get 0 empty = 0.
+  Proof. reflexivity. Qed.
+
+  Example ex2 : get 0 (set 0 3 empty) = 3.
+  Proof. reflexivity. Qed.
+
+  Example ex3 : get 1 (set 0 3 empty) = 0.
+  Proof. reflexivity. Qed.
 End NatFunTableExamples.
 
 (** [] *)
@@ -195,26 +210,29 @@ Module ListsTable (VT : ValType) <: Table.
 
   Definition empty : table := [].
 
-  Fixpoint get (k : key) (t : table) : V
-    (* REPLACE THIS LINE WITH ":= _your_definition_ ." *). Admitted.
+  Fixpoint get (k : key) (t : table) : V :=
+    match t with
+    | [] => default
+    | (hk, hv) :: t => if hk =? k then hv else get k t
+    end.
 
-  Definition set (k : key) (v : V) (t : table) : table
-    (* REPLACE THIS LINE WITH ":= _your_definition_ ." *). Admitted.
+  Definition set (k : key) (v : V) (t : table) : table := (k, v) :: t.
 
   Theorem get_empty_default: forall (k : key),
       get k empty = default.
-  Proof.
-    (* FILL IN HERE *) Admitted.
+  Proof. intros. reflexivity. Qed.
 
   Theorem get_set_same: forall (k : key) (v : V) (t : table),
       get k (set k v t) = v.
   Proof.
-    (* FILL IN HERE *) Admitted.
+    intros. unfold get, set. bdall.
+  Qed.
 
   Theorem get_set_other: forall (k k' : key) (v : V) (t : table),
       k <> k' -> get k' (set k v t) = get k' t.
   Proof.
-    (* FILL IN HERE *) Admitted.
+    intros. unfold get, set. bdall.
+  Qed.
 
 End ListsTable.
 
@@ -227,16 +245,13 @@ Module StringListsTableExamples.
   Open Scope string_scope.
 
   Example ex1 : get 0 empty = "".
-  Proof.
-    (* FILL IN HERE *) Admitted.
-
+  Proof. reflexivity. Qed.
+  
   Example ex2 : get 0 (set 0 "A" empty) = "A".
-  Proof.
-    (* FILL IN HERE *) Admitted.
+  Proof. reflexivity. Qed.
 
   Example ex3 : get 1 (set 0 "A" empty) = "".
-  Proof.
-    (* FILL IN HERE *) Admitted.
+  Proof. reflexivity. Qed.
 
 End StringListsTableExamples.
 
@@ -352,6 +367,21 @@ Module TreeETable_first_attempt (VT : ValType) <: ETable_first_attempt.
     apply Hcomplete with default.
     - (** Stuck! We don't know that [t] satisfies the BST invariant. *)
   Admitted.
+  
+  Theorem elements_complete' : forall (k : key) (v : V) (t : table),
+      bound k t = true ->
+      get k t = v ->
+      In (k, v) (elements t).
+  Proof.
+    intros k v t Hbound Hlookup. unfold get in Hlookup.
+    (** [pose proof t as H] is equivalent to [assert (H : ...the type
+        of t...). { apply t. }] but saves some keystrokes. *)
+    pose proof (SearchTree.elements_complete) as Hcomplete.
+    unfold elements_complete_spec in Hcomplete.
+    apply Hcomplete with default.
+    - unfold bound in Hbound. auto.
+    - auto.
+  Qed.
 
   Theorem elements_correct : forall (k : key) (v : V) (t : table),
       In (k, v) (elements t) ->
@@ -501,6 +531,8 @@ Module StringTreeETableExample.
   Qed.
 
 End StringTreeETableExample.
+
+(* FILL (I've read to here...) *)
 
 (* ################################################################# *)
 (** * Encapsulation with the Coq Module System (Advanced) *)
